work on disk io stuff; work on fractional foundation

examples/scache/Cache.i.dfy
@@ -20,6 +20,58 @@ module CacheImpl {
 
   linear datatype NullGhostType = NullGhostType
 
+  datatype Cache = Cache(
+    data: seq<Ptr>,
+    disk_idx_of_entry: seq<Ptr>,
+
+    status: seq<AtomicStatus>,
+    read_refcounts: seq<seq<AtomicRefcount>>,
+
+    cache_idx_of_page: seq<AtomicIndexLookup>,
+
+    global_clockpointer: Atomic<uint32, NullGhostType>
+  )
+  {
+    function method key(i: int) : RWLock.Key
+    requires 0 <= i < |this.data|
+    requires 0 <= i < |this.disk_idx_of_entry|
+    {
+      RWLock.Key(this.data[i], this.disk_idx_of_entry[i], i)
+    }
+
+    predicate Inv()
+    {
+      && |this.data| == CACHE_SIZE
+      && |this.disk_idx_of_entry| == CACHE_SIZE
+      && |this.status| == CACHE_SIZE
+      && (forall i | 0 <= i < CACHE_SIZE ::
+         atomic_status_inv(this.status[i], this.key(i)))
+      && |this.read_refcounts| == NUM_THREADS
+      && (forall j | 0 <= j < NUM_THREADS ::
+          |this.read_refcounts[j]| == CACHE_SIZE)
+      && (forall j, i | 0 <= j < NUM_THREADS && 0 <= i < CACHE_SIZE ::
+          atomic_refcount_inv(this.read_refcounts[j][i], this.key(i), j))
+      && |this.cache_idx_of_page| == NUM_DISK_PAGES
+      && (forall d | 0 <= d < NUM_DISK_PAGES ::
+          atomic_index_lookup_inv(this.cache_idx_of_page[d], d))
+    }
+  }
+
+  datatype LocalState = LocalState(
+    t: int,
+    chunk_idx: uint64
+  )
+  {
+    predicate WF()
+    {
+      && 0 <= this.chunk_idx as int < NUM_CHUNKS
+      && 0 <= t < NUM_THREADS
+    }
+  }
+
+  ////////////////////////////////////////
+  //// IO stuff
+
   datatype IOSlotInfo =
     | IOSlotUnused
     | IOSlotWrite(cache_idx: uint64)
@@ -53,11 +105,17 @@ module CacheImpl {
       linear q: RWLock.R,
       /*readonly*/ linear cache_entry: CacheResources.R,
       /*readonly*/ linear idx: Deref<int>)
-  /*{
-    predicate WF(addr: uint64)
+  {
+    predicate WF(c: Cache, cache_idx: int)
+    requires c.Inv()
     {
+      && 0 <= cache_idx < CACHE_SIZE
+      && this.q == RWLock.Internal(RWLock.WriteBackObtained(c.key(cache_idx)))
+      && this.cache_entry.CacheEntry?
+      && this.cache_entry.cache_idx == cache_idx
+      && this.idx.ptr == c.disk_idx_of_entry[cache_idx]
     }
-  }*/
+  }
 
   linear datatype LoadGhostState = LoadGhostState
 
@@ -74,86 +132,67 @@ module CacheImpl {
     linear read: LinearMap<Ptr, LoadGhostStateWithSlot>
   )
 
+  predicate WriteTaskInv(task: PendingWriteTask, g: WritebackGhostStateWithSlot, c: Cache)
+  requires c.Inv()
+  {
+    && g.info.v.IOSlotWrite?
+    && var cache_idx := g.info.v.cache_idx as int;
+    && g.g.WF(c, cache_idx)
+    && task.ptr == c.data[cache_idx]
+  }
+
+  predicate ReadTaskInv(task: PendingReadTask, g: LoadGhostStateWithSlot, c: Cache)
+  requires c.Inv()
+  {
+    true
+  }
+
   predicate WriteMapInv(
     writeTasks: map<Ptr, PendingWriteTask>,
-    writes: map<Ptr, WritebackGhostStateWithSlot>)
+    writes: map<Ptr, WritebackGhostStateWithSlot>,
+    c: Cache)
+  requires c.Inv()
   {
-    && (forall ptr | ptr in writeTasks :: ptr in writes)
+    && (forall ptr | ptr in writeTasks :: ptr in writes
+        && WriteTaskInv(writeTasks[ptr], writes[ptr], c))
     && (forall ptr | ptr in writes :: ptr in writeTasks)
   }
 
   predicate ReadMapInv(
     readTasks: map<Ptr, PendingReadTask>,
-    read: map<Ptr, LoadGhostStateWithSlot>)
+    read: map<Ptr, LoadGhostStateWithSlot>,
+    c: Cache)
+  requires c.Inv()
   {
-    && (forall ptr | ptr in readTasks :: ptr in read)
+    && (forall ptr | ptr in readTasks :: ptr in read
+        && ReadTaskInv(readTasks[ptr], read[ptr], c))
     && (forall ptr | ptr in read :: ptr in readTasks)
   }
 
-  predicate DIInvGhost(v: PendingTaskSet, g: DIGhost)
+  predicate DIInvGhost(v: PendingTaskSet, g: DIGhost, c: Cache)
+  requires c.Inv()
   {
-    && WriteMapInv(v.writeTasks, map_of(g.write))
-    && ReadMapInv(v.readTasks, map_of(g.read))
+    && WriteMapInv(v.writeTasks, map_of(g.write), c)
+    && ReadMapInv(v.readTasks, map_of(g.read), c)
   }
 
-  predicate DIInv(di: DiskInterface<DIGhost>)
+  predicate DIInv(di: DiskInterface<DIGhost>, c: Cache)
+  requires c.Inv()
   {
     forall v, g ::
-      disk_interface_inv(di, v, g) <==> DIInvGhost(v, g)
+      disk_interface_inv(di, v, g) <==> DIInvGhost(v, g, c)
   }
 
-  datatype Cache = Cache(
-    data: seq<Ptr>,
-    disk_idx_of_entry: seq<Ptr>,
-
-    status: seq<AtomicStatus>,
-    read_refcounts: seq<seq<AtomicRefcount>>,
-
-    cache_idx_of_page: seq<AtomicIndexLookup>,
-
-    global_clockpointer: Atomic<uint32, NullGhostType>,
-
+  datatype IOHandle = IOHandle(
     io_slots: seq<IOSlot>,
-    disk_interface: DiskInterface<DIGhost>
-  )
+    disk_interface: DiskInterface<DIGhost>)
   {
-    function method key(i: int) : RWLock.Key
-    requires 0 <= i < |this.data|
-    requires 0 <= i < |this.disk_idx_of_entry|
+    predicate Inv(c: Cache)
     {
-      RWLock.Key(this.data[i], this.disk_idx_of_entry[i], i)
+      && c.Inv()
+      && |this.io_slots| == NUM_IO_SLOTS
+      && (forall i | 0 <= i < |this.io_slots| :: this.io_slots[i].WF())
+      && DIInv(this.disk_interface, c)
     }
-  }
-
-  datatype LocalState = LocalState(
-    t: int,
-    chunk_idx: uint64
-  )
-  {
-    predicate WF()
-    {
-      && 0 <= this.chunk_idx as int < NUM_CHUNKS
-      && 0 <= t < NUM_THREADS
-    }
-  }
-
-  predicate Inv(c: Cache)
-  {
-    && |c.data| == CACHE_SIZE
-    && |c.disk_idx_of_entry| == CACHE_SIZE
-    && |c.status| == CACHE_SIZE
-    && (forall i | 0 <= i < CACHE_SIZE ::
-       atomic_status_inv(c.status[i], c.key(i)))
-    && |c.read_refcounts| == NUM_THREADS
-    && (forall j | 0 <= j < NUM_THREADS ::
-        |c.read_refcounts[j]| == CACHE_SIZE)
-    && (forall j, i | 0 <= j < NUM_THREADS && 0 <= i < CACHE_SIZE ::
-        atomic_refcount_inv(c.read_refcounts[j][i], c.key(i), j))
-    && |c.cache_idx_of_page| == NUM_DISK_PAGES
-    && (forall d | 0 <= d < NUM_DISK_PAGES ::
-        atomic_index_lookup_inv(c.cache_idx_of_page[d], d))
-    && |c.io_slots| == NUM_IO_SLOTS
-    && (forall i | 0 <= i < |c.io_slots| :: c.io_slots[i].WF())
-    && DIInv(c.disk_interface)
   }
 }
