examples/refcounter2/Frac.s.dfy
@@ -1,0 +1,26 @@
+include "Rational.s.dfy"
+
+module FracLogic {
+  import opened Rationals
+
+  linear datatype Frac<V> = Frac(linear v: V, r: PositiveRational)
+
+  function method {:extern} borrow<V>(shared frac: Frac<V>) : (shared v : V)
+  ensures v == frac.v
+
+  function method {:extern} exc<V>(linear frac: Frac<V>) : (linear v: V)
+  requires frac.r == one()
+  ensures v == frac.v
+
+  function method {:extern} wrap<V>(linear v: V) : (linear frac : Frac<V>)
+  ensures frac == Frac(v, one())
+
+  function method {:extern} frac_split<V>(
+      linear f: Frac<V>,
+      ghost r: PositiveRational)
+    : (linear res: (Frac<V>, Frac<V>))
+  requires Rationals.lt(r, f.r)
+  ensures res.0 == Frac(f.v, r)
+  ensures res.1 == Frac(f.v, Rationals.minus(f.r, r))
+
+}
