examples/refcounter2/RationalUtil.i.dfy
@@ -1,0 +1,7 @@
+module RationalUtil {
+  lemma in_between(lower: PositiveRational, upper: PositiveRational)
+  returns (mid: PositiveRational)
+  requires lt(lower, upper)
+  ensures lt(lower, mid)
+  ensures lt(mid, upper)
+}
