examples/refcounter2/ResourceBuilder.s.dfy
@@ -1,0 +1,153 @@
+include "Frac.s.dfy"
+include "ResourceSpec.s.dfy"
+include "../../lib/Base/Options.s.dfy"
+
+abstract module ResourceBuilder refines ResourceSpec {
+  import FracLogic
+  import Rationals
+  import opened Options
+
+  type V(==,!new)
+
+  /*
+   * User-provided properties
+   */
+
+  type Q
+  function qconst(v: V) : Q
+  function qexc(v: V) : Q
+  function qconst_v(q: Q) : Option<V>
+
+  datatype Variables = Variables(m: multiset<Q>, saved: multiset<V>)
+  predicate Init(s: Variables)
+  predicate transform(a: multiset<Q>, b: multiset<Q>)
+
+  predicate NewExc(s: Variables, s': Variables)
+  {
+    exists v ::
+      && s'.saved == s.saved + multiset{v}
+      && s'.m == s.m + multiset{Exc(v)}
+  }
+
+  predicate InternalStep(s: Variables, s': Variables)
+  {
+    && s'.saved == s.saved
+    && (exists a, b, c ::
+      s.m == a + c && s'.m == b + c && transform(a, b))
+  }
+
+  predicate QNext(s: Variables, s': Variables)
+  {
+    || NewExc(s, s')
+    || NewExc(s', s)
+    || InternalStep(s, s')
+  }
+
+  predicate QInv(s: Variables)
+
+  lemma InitImpliesQInv(s: Variables)
+  requires Init(s)
+  ensures QInv(s)
+
+  lemma NextPreservesQInv(s: Variables, s': Variables)
+  requires QInv(s)
+  requires QNext(s, s')
+  ensures QInv(s')
+
+  lemma QInvWorksConst(s: Variables, v: V)
+  requires QInv(s)
+  requires qconst(v) in s.m
+  ensures v in s.saved
+
+  lemma QInvWorksExc(s: Variables, v: V)
+  requires QInv(s)
+  requires qexc(v) in s.m
+  ensures v in s.saved
+
+  /*
+   * Const logic
+   */
+
+  datatype R =
+    | RG(s: Variables, fracs: map<V, multiset<RationalFraction>>)
+    | RFrac(v: V, r: Rationals.PositiveRational)
+    | Internal(q: Q)
+
+  linear datatype PreConst = Const(
+      linear rf: FracLogic.Frac<V>,
+      linear r: R)
+  {
+    function value() : V {
+      this.rf.v
+    }
+
+    predicate WF() {
+      && this.r == RFrac(this.rf.v, this.rf.r)
+    }
+  }
+
+  type Const = c : PreConst | c.WF()
+      witness (assume false; var c:PreConst :| true; c) // XXX
+
+  function method borrow(shared con: Const) : (shared v : V)
+  {
+    FracLogic.borrow(con.rf)
+  }
+
+  linear datatype G = G(store: LinearMap<V, Frac<V>>, state: R)
+
+  predicate HasQuote(store: LinearMap<V, Frac<V>>, m: multiset<V>, v: V)
+  {
+    var n := CountValue(m, v);
+    (n > 0 ==> 
+      && v in store
+      && store[v].v == v
+      && Rational.lt(Rational.of_nat(n-1), store[v].r)
+    )
+  }
+
+  predicate GInv(g: G)
+  {
+    && g.state.RG?
+    && QInv(g.state.s)
+    && (forall v :: HasQuota(store, state.saved, v))
+  }
+
+  method unsafe_obtain() returns (linear g: G)
+  ensures GInv(g)
+
+  method unsafe_dispose(linear g: G)
+  requires GInv(g)
+
+  method acquire_const(linear r: R)
+  returns (linear c: Const)
+  requires r.Internal? && qconst_v(r.q).Some?
+  ensures c.value() == qconst_v(r.q).value
+  {
+    linear var g := unsafe_obtain();
+
+    linear var G(store, state) := g;
+
+    var v := qconst_v(r.q);
+
+    var count := CountValue(state.s.saved, qconst_v(r.q));
+    CountValue_ge_1(state.s.saved, qconst_v(r.q));
+    assert count > 0;
+
+    var mid := RationalUtil.in_between(lower, upper);
+
+    linear var store', v_frac := LinearMap.remove(store, v);
+    linear var (v_frac', v_frac_lend) := FracLogic.frac_split(v_frac, mid);
+    store := LinearMap.add(v, v_frac');
+
+    linear var state', frac_tracker := transform_1_2(state,
+        state.(fracs := state.fracs[v := state.fracs[v] + multiset{v_frac_lend}]),
+        RFrac(v, v_frac_lend));
+
+    c := Const(
+      v_frac_lend,
+      frac_tracker);
+
+    unsafe_dispose(G(store, state'));
+  }
+}
