examples/scache/CacheIO.i.dfy
@@ -10,54 +10,59 @@ module CacheIOImpl {
   import LinearMaps
   import opened DiskInterfaceSpec
 
-  method get_free_io_slot(c: Cache)
+  method get_free_io_slot(c: Cache, io: IOHandle)
   returns (idx: uint64, linear access: IOSlotAccess)
-  requires Inv(c)
+  requires io.Inv(c)
   ensures 0 <= idx as int < NUM_IO_SLOTS
-  ensures is_slot_access(c.io_slots[idx], access)
+  ensures is_slot_access(io.io_slots[idx], access)
 
   method disk_writeback_async(
       c: Cache,
+      io: IOHandle,
       disk_idx: uint64,
       cache_idx: uint64,
       /*readonly*/ linear contents: Ptrs.ArrayDeref<byte>,
       linear g: WritebackGhostState,
       linear ticket: DiskWriteTicket)
-  requires Inv(c)
+  requires c.Inv()
+  requires io.Inv(c)
   requires 0 <= cache_idx as int < CACHE_SIZE
   requires 0 <= disk_idx as int < NUM_DISK_PAGES
   requires contents.ptr == c.data[cache_idx]
   requires |contents.s| == 4096
   requires ticket == DiskWriteTicket(disk_idx * 4096, contents.s)
+  requires g.WF(c, cache_idx as int)
   {
     var idx;
     linear var access;
-    idx, access := get_free_io_slot(c);
+    idx, access := get_free_io_slot(c, io);
     linear var IOSlotAccess(aiocb, info) := access;
 
-    ptr_write(c.io_slots[idx].aiocb_ptr,
+    ptr_write(io.io_slots[idx].aiocb_ptr,
         inout aiocb,
         aiocb_constructor(disk_idx * 4096, c.data[cache_idx], 4096));
 
-    ptr_write(c.io_slots[idx].info_ptr,
+    ptr_write(io.io_slots[idx].info_ptr,
         inout info,
         IOSlotWrite(cache_idx));
 
     var old_v, new_v;
     linear var old_g;
     old_v, new_v, old_g := async_write(
-        c.disk_interface,
-        c.io_slots[idx].aiocb_ptr,
+        io.disk_interface,
+        io.io_slots[idx].aiocb_ptr,
         aiocb,
         contents,
         ticket);
     ///////////////////////////////////////////////////////////////////
     linear var DIGhost(writeMap, readMap) := old_g;
-    writeMap := LinearMaps.add(writeMap, c.io_slots[idx].aiocb_ptr,
+    writeMap := LinearMaps.add(writeMap, io.io_slots[idx].aiocb_ptr,
         WritebackGhostStateWithSlot(info, g));
     linear var new_g := DIGhost(writeMap, readMap);
+    assert WriteTaskInv(new_v.writeTasks[io.io_slots[idx].aiocb_ptr],
+        WritebackGhostStateWithSlot(info, g), c);
     ///////////////////////////////////////////////////////////////////
-    disk_interface_op_cleanup(c.disk_interface, new_v, new_g);
+    disk_interface_op_cleanup(io.disk_interface, new_v, new_g);
     ///////////////////////////////////////////////////////////////////
   }
 
@@ -75,13 +80,16 @@ module CacheIOImpl {
   ensures stub == DiskReadStub(addr, contents.s)
 
 
-  /*method disk_writeback_callback(
+  method disk_writeback_callback(
       c: Cache,
       addr: uint64,
       /*readonly*/ linear contents: Ptrs.ArrayDeref<byte>,
       linear g: CacheIOImpl.WritebackGhostState,
       linear stub: CacheResources.R)
-  requires Inv(c)
+  requires c.Inv()
   requires stub == CacheResources.DiskWriteStub(addr)
-  requires g.WF(addr)*/
+  requires g.WF(addr)
+  {
+    
+  }
 }
